code/mpfr/MPFR.Lib.fst
@@ -156,12 +156,12 @@ let mpfr_LIMB_MASK s =
     let lsh = 1uL <<^ s in
     lemma_pow2_small_mod (U32.v s) 64;
     lsh -^ 1uL
-
+    
 val mpfr_LIMB_HIGHBIT: s:u64{v s = pow2 63}
 let mpfr_LIMB_HIGHBIT =
-    assert_norm(pow2_n #64 63 == v 0x8000000000000000uL);
+    assert_norm(pow2_n #64 63 = v 0x8000000000000000uL);
     0x8000000000000000uL
-
+    
 assume val gmpfr_emax: mpfr_exp_t
 assume val gmpfr_flags: i32
 
